genWhile_ind proof goes through with trivial admits
This took way too long....

coq/LLVMGen/Correctness_While.v
@@ -69,14 +69,14 @@ Notation "'(Z)' x" := (Z.of_nat x) (at level 10).
 
 (* TODO: Move to Vellvm Denotation_Theory.v? *)
 
-Definition block_ids {T : Set} (b : list ((LLVMAst.block T))) :=
-  fold_left (fun (acc : list block_id) (bk : LLVMAst.block T) => (acc ++ [blk_id bk])%list) b [].
+(* Definition block_ids {T : Set} (b : list ((LLVMAst.block T))) := *)
+(*   fold_left (fun (acc : list block_id) (bk : LLVMAst.block T) => (acc ++ [blk_id bk])%list) b []. *)
 
 (* IY: Why isn't it the below, instead? It looks like outputs etc. also have use
    fold_left instead of map (in Vellvm - Denotation_Theory.v), which feels super
    awkward. Following Vellvm conventions for now. *)
-Definition block_ids' {T : Set} (b : list ((LLVMAst.block T))) :=
-  map (@blk_id T).
+Definition block_ids {T : Set} (b : list ((LLVMAst.block T))) :=
+  map (@blk_id T) b.
 
 Definition disjoint_bid_blocks {T : Set} (b b' : list ((LLVMAst.block T))) :=
   block_ids b ⊍ block_ids b'.
@@ -107,90 +107,119 @@ Proof.
     reflexivity.
 Qed.
 
-(* IY: The more general statement should be In being injective over List.map,
-   but it's stated like this here because we're using fold_left *)
-Lemma In_inj_block_ids :
-  forall T x (b : list (LLVMAst.block T)), In x b -> In (blk_id x) (block_ids b).
-Proof.
-  intros. revert H. revert x. induction b.
-  - intros. inversion H.
-  - intros. unfold block_ids. cbn.
-    rewrite fold_left_acc_app. rewrite <-list_cons_app.
-    cbn in H. destruct H. cbn. left. rewrite H. reflexivity.
-    cbn. right. apply IHb. auto.
-Qed.
+(* (* IY: The more general statement should be In being injective over List.map, *)
+(*    but it's stated like this here because we're using fold_left *) *)
+(* Lemma In_inj_block_ids : *)
+(*   forall T x (b : list (LLVMAst.block T)), In x b -> In (blk_id x) (block_ids b). *)
+(* Proof. *)
+(*   intros. revert H. revert x. induction b. *)
+(*   - intros. inversion H. *)
+(*   - intros. unfold block_ids. cbn. *)
+(*     rewrite fold_left_acc_app. rewrite <-list_cons_app. *)
+(*     cbn in H. destruct H. cbn. left. rewrite H. reflexivity. *)
+(*     cbn. right. apply IHb. auto. *)
+(* Qed. *)
 
-Definition imp_rel {A B : Type} (R S: A -> B -> Prop): Prop :=
-  forall a b, R a b -> S a b.
+(* Definition imp_rel {A B : Type} (R S: A -> B -> Prop): Prop := *)
+(*   forall a b, R a b -> S a b. *)
 
 
-Definition stable_exp_local (R: Rel_cfg) : Prop :=
-    forall memH memV ρ1 ρ2 g,
-      R memH (memV, (ρ1, g)) ->
-      ρ1 ⊑ ρ2 ->
-      R memH (memV, (ρ2, g)).
+(* Definition stable_exp_local (R: Rel_cfg) : Prop := *)
+(*     forall memH memV ρ1 ρ2 g, *)
+(*       R memH (memV, (ρ1, g)) -> *)
+(*       ρ1 ⊑ ρ2 -> *)
+(*       R memH (memV, (ρ2, g)). *)
 
-Lemma disjoint_bid_neq {T : Set} (b b' : list (LLVMAst.block T)) :
-  disjoint_bid_blocks b b' ->
-  forall x x', In x b -> In x' b' -> blk_id x ≢ blk_id x'.
-Proof.
-  intros.
-  do 2 red in H.
-  specialize (H (blk_id x) (blk_id x')).
-  apply H; apply In_inj_block_ids; auto.
-Qed.
+(* Lemma disjoint_bid_neq {T : Set} (b b' : list (LLVMAst.block T)) : *)
+(*   disjoint_bid_blocks b b' -> *)
+(*   forall x x', In x b -> In x' b' -> blk_id x ≢ blk_id x'. *)
+(* Proof. *)
+(*   intros. *)
+(*   do 2 red in H. *)
+(*   specialize (H (blk_id x) (blk_id x')). *)
+(*   apply H; apply In_inj_block_ids; auto. *)
+(* Qed. *)
 
-Lemma find_block_ineq :
-  ∀ (T : Set) (x : block_id) (b bs : list (LLVMAst.block T)) e,
-    disjoint_bid_blocks b bs ->
-    find_block T bs x ≡ Some e -> find_block T (b ++ bs) x ≡ Some e.
+(* Lemma find_block_ineq : *)
+(*   ∀ (T : Set) (x : block_id) (b bs : list (LLVMAst.block T)) e, *)
+(*     disjoint_bid_blocks b bs -> *)
+(*     find_block T bs x ≡ Some e -> find_block T (b ++ bs) x ≡ Some e. *)
+(* Proof. *)
+(*   intros. *)
+(*   induction b. *)
+(*   - intros. rewrite app_nil_l. apply H0. *)
+(*   - intros. *)
+(*     rewrite list_cons_app. *)
+(*     rewrite <- app_assoc. *)
+(*     rewrite <- list_cons_app. *)
+(*     cbn. *)
+(*     assert (blk_id a ≢ x). *)
+(*     assert (H' := H0). *)
+(*     apply find_some in H0. destruct H0. *)
+(*     assert (In a (a :: b)). { red. left. reflexivity. } *)
+(*     destruct (Eqv.eqv_dec_p (blk_id e) x). 2 : inversion H1. *)
+(*     rewrite <- e0. *)
+(*     eapply disjoint_bid_neq; eauto. *)
+(*     assert (not (Eqv.eqv (blk_id a) x)). red. intros. apply H1. rewrite H2. reflexivity. *)
+(*     unfold Eqv.eqv_dec_p. eapply rel_dec_neq_false in H2. 2 : typeclasses eauto. *)
+(*     setoid_rewrite H2. apply IHb. *)
+(*     red. red in H. *)
+(*     eapply Coqlib.list_disjoint_cons_left. *)
+(*     rewrite list_cons_app in H. *)
+(*     clear H0 IHb H1 H2. induction b. cbn. rewrite app_nil_r in H. *)
+(*     apply H. red. intros. red in H. apply H. 2 : auto. *)
+(*     eapply Permutation.Permutation_in. 2: apply H0. *)
+(*     clear H IHb H0 H1. *)
+(*     remember (a0 :: b). clear Heql. *)
+(*     induction l. cbn. auto. *)
+(*     cbn. cbn in IHl. eapply Permutation.perm_trans. *)
+(*     rewrite list_cons_app. *)
+(*     rewrite Permutation.Permutation_app_swap. apply Permutation.Permutation_refl. *)
+(*     pose proof @fold_left_acc_app . *)
+(*     specialize (H _ _ l (fun x => [blk_id x])). cbn in H. *)
+(*     assert ( *)
+(*     (fold_left (λ (acc : list block_id) (bk : LLVMAst.block T), (acc ++ [blk_id bk])%list) l [blk_id a1] ++ *)
+(*                [blk_id a]) ≡ *)
+(*      ([blk_id a1] ++ fold_left (λ (acc : list block_id) (bk : LLVMAst.block T), acc ++ [blk_id bk]) l [ ]) ++ *)
+(*      [blk_id a])%list. rewrite H. reflexivity. rewrite H0. *)
+(*     assert ( *)
+(*     (fold_left (λ (acc : list block_id) (bk : LLVMAst.block T), (acc ++ [blk_id bk])%list) l *)
+(*        [blk_id a; blk_id a1]) ≡ *)
+(*      ([blk_id a; blk_id a1] ++ fold_left (λ (acc : list block_id) (bk : LLVMAst.block T), acc ++ [blk_id bk]) l [ ])%list). *)
+(*     rewrite H; reflexivity. *)
+(*     rewrite H1. clear H0 H1. eapply Permutation.perm_trans. *)
+(*     apply Permutation.Permutation_app_swap. cbn. *)
+(*     apply Permutation.Permutation_refl. *)
+(* Qed. *)
+
+
+(* All labels in a list of blocks are distinct *)
+Definition blk_id_norepet {T} (bks : list (LLVMAst.block T)) :=
+  Coqlib.list_norepet (map blk_id bks).
+
+Lemma blk_id_norepet_find_block {T} :
+  forall (bks : list (LLVMAst.block T)), blk_id_norepet bks ->
+  forall x b bs e, (bks ≡ b ++ bs)%list -> find_block T bs x ≡ Some e -> find_block T (b ++ bs) x ≡ Some e.
 Proof.
   intros.
   induction b.
-  - intros. rewrite app_nil_l. apply H0.
+  - intros. rewrite app_nil_l. auto.
   - intros.
     rewrite list_cons_app.
     rewrite <- app_assoc.
     rewrite <- list_cons_app.
     cbn.
     assert (blk_id a ≢ x).
-    assert (H' := H0).
-    apply find_some in H0. destruct H0.
+    assert (H' := H1).
+    apply find_some in H1. destruct H1.
     assert (In a (a :: b)). { red. left. reflexivity. }
-    destruct (Eqv.eqv_dec_p (blk_id e) x). 2 : inversion H1.
+    destruct (Eqv.eqv_dec_p (blk_id e) x). 2 : inversion H3.
     rewrite <- e0.
-    eapply disjoint_bid_neq; eauto.
-    assert (not (Eqv.eqv (blk_id a) x)). red. intros. apply H1. rewrite H2. reflexivity.
-    unfold Eqv.eqv_dec_p. eapply rel_dec_neq_false in H2. 2 : typeclasses eauto.
-    setoid_rewrite H2. apply IHb.
-    red. red in H.
-    eapply Coqlib.list_disjoint_cons_left.
-    rewrite list_cons_app in H.
-    clear H0 IHb H1 H2. induction b. cbn. rewrite app_nil_r in H.
-    apply H. red. intros. red in H. apply H. 2 : auto.
-    eapply Permutation.Permutation_in. 2: apply H0.
-    clear H IHb H0 H1.
-    remember (a0 :: b). clear Heql.
-    induction l. cbn. auto.
-    cbn. cbn in IHl. eapply Permutation.perm_trans.
-    rewrite list_cons_app.
-    rewrite Permutation.Permutation_app_swap. apply Permutation.Permutation_refl.
-    pose proof @fold_left_acc_app .
-    specialize (H _ _ l (fun x => [blk_id x])). cbn in H.
-    assert (
-    (fold_left (λ (acc : list block_id) (bk : LLVMAst.block T), (acc ++ [blk_id bk])%list) l [blk_id a1] ++
-               [blk_id a]) ≡
-     ([blk_id a1] ++ fold_left (λ (acc : list block_id) (bk : LLVMAst.block T), acc ++ [blk_id bk]) l [ ]) ++
-     [blk_id a])%list. rewrite H. reflexivity. rewrite H0.
-    assert (
-    (fold_left (λ (acc : list block_id) (bk : LLVMAst.block T), (acc ++ [blk_id bk])%list) l
-       [blk_id a; blk_id a1]) ≡
-     ([blk_id a; blk_id a1] ++ fold_left (λ (acc : list block_id) (bk : LLVMAst.block T), acc ++ [blk_id bk]) l [ ])%list).
-    rewrite H; reflexivity.
-    rewrite H1. clear H0 H1. eapply Permutation.perm_trans.
-    apply Permutation.Permutation_app_swap. cbn.
-    apply Permutation.Permutation_refl.
-Qed.
+    red in H.
+Admitted.
+
+
+(* list_nopet -> then we can use find_block to find anything  *)
 
 (* Useful lemmas about rcompose. TODO: Move? *)
 Lemma rcompose_eq_r :
@@ -230,42 +259,22 @@ Lemma find_block_label_in_blocks :
 Proof.
 Admitted.
 
-Lemma body_blocks_from_entry_eq:
-  forall (prefix : string)
-    (loopvar : raw_id)            (* lvar storing the loop index *)
-    (loopcontblock : block_id)    (* reentry point from the body back to the loop *)
-    (body_entry : block_id)       (* entry point of the body *)
-    (body_blocks : list (LLVMAst.block typ)) (* (llvm) body to be iterated *)
-    (nextblock : block_id)        (* exit point of the overall loop *)
-    (entry_id : block_id)         (* entry point of the overall loop *)
-    (s1 s2 : IRState)
-    (n : nat)
-    (bks : list (LLVMAst.block typ)),
-
-    In body_entry (block_ids body_blocks) ->
-
-    (* Generation of the LLVM code wrapping the loop around bodyV *)
-    genWhileLoop prefix (EXP_Integer 0%Z) (EXP_Integer (Z.of_nat n))
-                       loopvar loopcontblock body_entry body_blocks [] nextblock s1
-                       ≡ inr (s2,(entry_id, bks)) ->
-
-    (* TODO: Add hypothesis about freshness/separation btw body_blocks and bks. *)
-
-    forall g l mV _label,
-      eutt Logic.eq
-      (with_err_LB (interp_cfg (denote_bks (convert_typ [ ] body_blocks) (_label, body_entry)) g l mV))
-      (with_err_LB (interp_cfg (denote_bks (convert_typ [ ] bks) (_label, body_entry)) g l mV)).
+Lemma denote_bks_prefix_ :
+  forall (prefix bks postfix : list (LLVMAst.block dtyp)) (from to: block_id),
+    In to (map blk_id bks) ->
+    (* All labels are distinct *)
+    Coqlib.list_norepet (map blk_id (prefix ++ bks ++ postfix)) ->
+    denote_bks (prefix ++ bks ++ postfix) (from, to) ≈
+               ITree.bind (denote_bks bks (from, to))
+               (fun x => match x with
+                      | inl x => denote_bks (prefix ++ bks ++ postfix) x
+                      | inr x => ret (inr x)
+                      end
+               ).
 Proof.
-  intros. unfold genWhileLoop in H0. cbn* in H0. simp.
-  rewrite list_cons_app.
-  rewrite convert_typ_block_app.
-  apply find_block_label_in_blocks in H. destruct H.
-  rewrite denote_bks_flow_right. 2 : admit. (* TODO: Freshness. *)
-
-  rewrite denote_bks_unfold_in.
-  2 : apply H.
-  cbn...
+  (* denote_bks_app denote_bks_cons *)
 Admitted.
+
 
 (* TODO: Freshness is stated in a somewhat ad-hoc way in here. Needs clean-up. *)
 Lemma genWhileLoop_ind:
@@ -280,22 +289,14 @@ Lemma genWhileLoop_ind:
     (bks : list (LLVMAst.block typ))
     (n : nat)                       (* Number of iterations *)
     (j : nat)                       (* Starting iteration *)
-    (BOUND : (n >= j))
+    (BOUND : n > j)
     (* Main relations preserved by iteration *)
     (I : nat -> mem_block -> Rel_cfg),
 
     In body_entry (block_ids body_blocks) ->
 
-    (* Uniqueness of identifiers *)
-    find_block dtyp (convert_typ [ ] body_blocks) loopcontblock ≡ None ->
-    find_block dtyp (convert_typ [ ] body_blocks) nextblock ≡ None ->
-    entry_id ≢ loopcontblock ->
-    entry_id ≢ nextblock ->
-    loopcontblock ≢ nextblock ->
-    (forall loop_id i i0,
-        incBlockNamed (prefix @@ "_entry") s1 ≡ inr (i, entry_id) ->
-        incBlockNamed (prefix @@ "_loop") i ≡ inr (i0, loop_id) ->
-        loop_id ≢ loopcontblock /\ loop_id ≢ nextblock) ->
+    (* All labels generated are distinct *)
+    blk_id_norepet bks ->
 
     (* Generation of the LLVM code wrapping the loop around bodyV *)
     genWhileLoop prefix (EXP_Integer 0%Z) (EXP_Integer (Z.of_nat n))
@@ -309,18 +310,17 @@ Lemma genWhileLoop_ind:
     (* We build weakening in the rule: the precondition implies the initial invariant
        and the final invariant implies the postcondition
      *)
-    (forall g l mV mH ymem k _label,
+    (forall g l mV mH ymem k _label _label',
 
         (conj_rel (I k ymem)
                   (fun _ '(_, (l, _)) => l @ loopvar ≡ Some (uvalue_of_nat k))
                   mH (mV,(l,g))) ->
         eutt
-          (
              (fun '(memH,vec') '(memV, (l, (g, x))) =>
                 l @ loopvar ≡ Some (uvalue_of_nat k) /\
-                I (S k) vec' memH (memV, (l, g))
-    ))
-          (with_err_RB (interp_Mem (bodyH k ymem) mH))
+                x ≡ inl (_label', loopcontblock) /\
+                I (S k) vec' memH (memV, (l, g)))
+          (with_err_RB (interp_Mem (bodyH (S k) ymem) mH))
           (with_err_LB (interp_cfg
                           (denote_bks (convert_typ [] body_blocks) (_label, body_entry)) g l mV))
     ) ->
@@ -328,30 +328,16 @@ Lemma genWhileLoop_ind:
     (* Invariant is stable under extending local state *)
     (forall k mH mV l l' g ymem, I k ymem mH (mV, (l, g)) -> l ⊑ l' -> I k ymem mH (mV, (l', g))) ->
 
-
     (* Main result. Need to know initially that P holds *)
     forall g l mV mH ymem _label,
-
-
-  (forall i i0 i1 i2 r r0 b0,
-      incBlockNamed (prefix @@ "_entry") s1 ≡ inr (i, entry_id) ->
-      incBlockNamed (prefix @@ "_loop") i ≡ inr (i0, b0) ->
-      incLocal i0 ≡ inr (i1, r) ->
-      incLocal i1 ≡ inr (i2, r0) ->
-
-      (alist_fresh r0
-        (alist_add (Name ((prefix @@ "_next_i") @@ string_of_nat (local_count i2)))
-          (UVALUE_I64 ((int64) ((Z) j) + (int64) 1)) l) /\
-            alist_fresh (Name ((prefix @@ "_next_i") @@ string_of_nat (local_count i2))) l)) ->
-
       (conj_rel
          (I j ymem)
-         (fun _ '(_, (l, _)) => l @ loopvar ≡ Some (uvalue_of_nat j))
+         (fun _ '(_, (l, _)) => l @ loopvar ≡ Some (uvalue_of_nat (j - 1)))
          mH (mV,(l,g))
       ) ->
       eutt (fun '(memH,vec') '(memV, (l, (g,x))) =>
-              (* l @ loopvar ≡ Some (uvalue_of_nat n) /\ *)
               x ≡ inl (loopcontblock, nextblock) /\
+              l @ loopvar ≡ Some (uvalue_of_nat n) /\
               I n vec' memH (memV,(l,g))
            )
            (with_err_RB (interp_Mem (build_vec_gen (S j) n bodyH ymem) mH))
@@ -359,25 +345,40 @@ Lemma genWhileLoop_ind:
                                                 (_label, loopcontblock)) g l mV)).
 
 Proof with rauto.
-  intros * BOUND * IN F0 F1 F2 F3 F4 F5 GEN.
+  intros * BOUND * IN UNIQUE_IDENTS GEN.
   unfold genWhileLoop in GEN. cbn* in GEN. simp.
   intros * HBODY STABLE.
-  remember (n - j) as k.
-  assert (JEQ: j ≡ n - k) by lia.
-  rewrite JEQ. clear BOUND Heqk JEQ j.
+  unfold build_vec_gen.
+  remember (n - S j) as k eqn:K_EQ.
+  assert (JEQ: S j ≡ n - k) by lia. rewrite JEQ.
+  assert (JEQ' : j ≡ (n -  S k )) by lia. rewrite JEQ' in *.
+  clear JEQ JEQ'.
 
-  generalize dependent k.
-  generalize dependent n.
-  induction k as [| k IH]; intros * FRESH PRE.
+  red in UNIQUE_IDENTS. cbn in UNIQUE_IDENTS. rewrite map_app in UNIQUE_IDENTS.
+  cbn in UNIQUE_IDENTS.
+  assert (MAP_CONV: forall bs, map blk_id bs ≡ map blk_id (convert_typ [] bs)). {
+    induction bs. cbn. reflexivity.
+    cbn. rewrite IHbs. reflexivity.
+  }
+  rewrite MAP_CONV in UNIQUE_IDENTS.
+
+  match goal with
+  | [ |- context[convert_typ [] (?a::?b::_ ++?c)]] => remember a as entry_bk;
+                                                       remember b as b0_bk;
+                                                       remember c as loopcont_bk
+  end.
+
+  induction k as [| k IH].
   - admit.
-  (* - cbn... *)
-  (*   (* LHS Helix simplification *) *)
-  (*   unfold build_vec_gen, build_vec_gen_aux. *)
-  (*   assert (n - S j ≡ 0) by lia. *)
-  (*   rewrite H. cbn. *)
+  (* - intros * (INV & LOOPVAR). *)
+  (*   (* admit. (* TODO: Redo base case with new unique ident property *) *) *)
   (*   cbn... *)
 
   (*   (* RHS Vellvm simplification *) *)
+  (*   subst. *)
+  (*   Arguments fmap /. *)
+  (*   Arguments Fmap_block /. *)
+  (*   cbn. intros. *)
   (*   rewrite denote_bks_unfold_in. *)
   (*   2 : { *)
   (*     rewrite find_block_ineq. rewrite find_block_ineq. *)
@@ -386,8 +387,10 @@ Proof with rauto.
   (*     cbn. unfold fmap, Fmap_block. cbn. rewrite find_block_eq. *)
   (*     reflexivity. cbn. reflexivity. *)
   (*     auto. *)
-  (*     cbn. eapply F5; eauto. *)
-  (*     cbn. auto. *)
+  (*     cbn. *)
+  (*     apply find_block_not_in_inputs. *)
+  (*     red. intros. inversion UNIQUE_IDENTS. subst. *)
+  (*     inversion H3. subst. admit. (* TODO: *) admit. admit. *)
   (*   } *)
   (*   cbn... *)
   (*   cbn... *)
@@ -400,7 +403,7 @@ Proof with rauto.
   (*   2 : { *)
   (*     cbn... *)
   (*     2 : { *)
-  (*       destruct PRE; eauto. *)
+  (*       eauto. *)
   (*     } *)
   (*     cbn... *)
   (*     unfold uvalue_to_dvalue_binop. *)
@@ -431,18 +434,7 @@ Proof with rauto.
   (*     match goal with *)
   (*     | [ |- ret (_, (_, (_, ?x))) ≈ Ret (_, (_, (_, ?x'))) ] => assert (x ≡ x') *)
   (*         end. *)
-  (*     unfold eval_int_icmp. cbn. *)
-  (*     assert ((int64) ((Z) j) + (int64) 1 < (int64) ((Z) n) ≡ false). { *)
-  (*       symmetry in EQ. rewrite Nat.sub_0_le in EQ. *)
-  (*       assert (j + 1 > n) by lia. *)
-  (*       apply gt_asym in H0. *)
-  (*       apply Bool.not_true_is_false. red. intros. apply H0. *)
-  (*       assert ((j + 1 < n -> n > j + 1)%nat). intros; lia. *)
-  (*       apply H2. clear H2. *)
-  (*       apply bounds_check_aux. auto. *)
-  (*     } *)
-  (*     rewrite H0. cbn. reflexivity. *)
-  (*     cbn. rewrite H0. reflexivity. *)
+  (*     admit. rewrite H. cbn. reflexivity. *)
   (*   } *)
   (*   cbn... subst. rewrite denote_bks_unfold_not_in. *)
   (*   2 : { *)
@@ -450,68 +442,110 @@ Proof with rauto.
   (*     rewrite convert_typ_block_app. rewrite find_block_none_app. *)
   (*     Opaque find_block. *)
   (*     cbn. unfold fmap, Fmap_block. cbn. rewrite find_block_ineq. *)
-  (*     apply find_block_nil. cbn. auto. auto. cbn. eapply F5; eauto. cbn. auto. *)
+  (*     apply find_block_nil. cbn. auto. auto. cbn. *)
+  (*     admit. admit. admit. admit. *)
   (*   } *)
   (*   cbn... apply eutt_Ret. *)
   (*   split. *)
   (*   + reflexivity. *)
-  (*   + *)
-  (*     eapply HBODY. destruct PRE. *)
-  (*     2 : { *)
-  (*       Unshelve. *)
-  (*       eapply sub_alist_add. cbn. *)
-  (*       eapply FRESH; eauto. *)
-  (*     } eapply HBODY. *)
-  (*     2 : { *)
-  (*       Unshelve. 2 : exact l. *)
-  (*       eapply sub_alist_add.  eapply FRESH; eauto. *)
-  (*     } *)
-  (*     assert (n <= j). lia. *)
-  (*     assert (n ≡ j). lia. *)
-  (*     rewrite H1. auto. *)
+  (*   + assert (NUM : n - 1 ≡ n - 0 - 1). lia. *)
+  (*     eapply STABLE. apply INV. *)
+  (*     red. intros. (* TODO: local freshness*) admit. *)
 
-  -
-    match goal with
-    | [ |- context[convert_typ _ ?l] ] => remember l as L
-    end.
+  - cbn in *. intros * (INV & LOOPVAR).
+    Arguments fmap /.
+    Arguments Fmap_block /.
+    cbn...
 
     (* RHS : Reducing RHS to apply Body Hypothesis *)
     (* First step : First, Check that k<n hence we do not exit, in order to jump back to bodyblock. *)
-    setoid_rewrite list_cons_app in HeqL.
-    subst.
+    rewrite list_cons_app.
     rewrite convert_typ_block_app.
     (* We ignore entry_id *)
-    rewrite denote_bks_flow_right.
-
-    match goal with
-    | [ |- context[convert_typ _ ?l] ] => remember l as L
-    end. setoid_rewrite list_cons_app in HeqL.
-    subst. rewrite convert_typ_block_app.
+    cbn. rewrite list_cons_app.
     rewrite denote_bks_unfold_in. cbn.
-    cbn...
+
+    (* START rewrite *)
+    rewrite bind_bind. rewrite bind_bind. rewrite interp_cfg_to_L3_bind.
+    rewrite translate_bind.
+    (* END rewrite *)
+
     2 : {
-      rewrite convert_typ_block_app.
+      match goal with
+      | [ |- find_block dtyp (_ ++ ?l) _ ≡ _ ] => remember l
+      end
+      .
+      rewrite list_cons_app in Heql0.
+      rewrite Heql0.
       rewrite app_assoc.
-      eapply find_block_ineq. admit.
-      cbn.
-      assert (loopcontblock ≡ loopcontblock) by reflexivity.
-      eapply rel_dec_eq_true in H. 2 : typeclasses eauto. setoid_rewrite H.
-      reflexivity.
+      rewrite app_assoc. erewrite blk_id_norepet_find_block. reflexivity.
+      2 : reflexivity. cbn. cbn in UNIQUE_IDENTS.
+      2 : {
+        cbn. subst.
+        assert (EQ: loopcontblock ≡ loopcontblock) by reflexivity.
+        eapply rel_dec_eq_true in EQ. 2 : typeclasses eauto. subst.
+        cbn. setoid_rewrite EQ. reflexivity.
+      }
+      red. cbn.
+      rewrite map_app. cbn. subst. cbn. 
+      apply UNIQUE_IDENTS.
     }
 
     (* Updating (loopvar <- S k) coming from loopcontblock. *)
     focus_single_step_v.
-    unfold fmap, Fmap_block. cbn. cbn... 
-    rewrite Heqi7. cbn...
+    cbn.
+
+    (* START rewrite *)
+    rewrite interp_cfg_to_L3_ret. rewrite translate_ret. rewrite bind_ret_l.
+    (* END rewrite *)
+
+    rewrite Heqi7.
+
+    (* START rewrite *)
+    rewrite bind_bind. rewrite interp_cfg_to_L3_bind.
+    rewrite translate_bind. cbn. rewrite interp_cfg_to_L3_ret.
+    rewrite translate_ret. rewrite bind_ret_l. rewrite bind_ret_l.
+    rewrite bind_bind. rewrite interp_cfg_to_L3_bind.
+    rewrite translate_bind. cbn.
+    (* END rewrite *)
+
     focus_single_step_v.
     Transparent denote_code.
     unfold denote_code. cbn. Opaque denote_code.
-    cbn... focus_single_step_v.
-    Transparent denote_instr. unfold denote_instr. cbn...
+
+    (* START rewrite *)
+    rewrite bind_bind. rewrite interp_cfg_to_L3_bind.
+    rewrite translate_bind. rewrite bind_bind.
+    (* END rewrite *)
+
+    focus_single_step_v.
+    Transparent denote_instr. unfold denote_instr.
     Opaque denote_instr.
-    2 : { destruct PRE as (INV & LOOPVAR). apply LOOPVAR. }
-    cbn. cbn...
+
+    (* START rewrite *)
+    setoid_rewrite interp_cfg_to_L3_bind. rewrite translate_bind.
+    rewrite bind_bind. cbn. (* This cbn takes so long.. *)
+    rewrite translate_bind. rewrite interp_cfg_to_L3_bind.
+    rewrite translate_bind. rewrite bind_bind.
+    rewrite translate_trigger. rewrite translate_trigger.
+    rewrite lookup_E_to_exp_E_Local.
+    rewrite subevent_subevent.
+    rewrite exp_E_to_instr_E_Local. rewrite subevent_subevent.
+    rewrite interp_cfg_to_L3_LR.
+    (* END rewrite *)
+
+    2 : { cbn... eauto. }
+    cbn.
+
+    (* START rewrite *)
+    rewrite translate_ret. rewrite bind_ret_l. rewrite translate_bind.
+    rewrite interp_cfg_to_L3_bind. rewrite translate_bind. rewrite bind_bind.
+    cbn...
+    (* END rewrite *)
+
     unfold uvalue_to_dvalue_binop. cbn. cbn...
+    unfold uvalue_to_dvalue. cbn.
+    cbn...
     rewrite interp_cfg_to_L3_LW. cbn...
 
     (* Simplifying until we get to the branching conditional statement. *)
@@ -523,56 +557,96 @@ Proof with rauto.
       setoid_rewrite lookup_alist_add_eq. reflexivity.
     }
     cbn. cbn...
-    rewrite interp_cfg_to_L3_LW. cbn. cbn...
+    rewrite interp_cfg_to_L3_LW. cbn.
+
+    (* START rewrite *)
+    rewrite translate_ret. rewrite bind_ret_l. rewrite interp_cfg_to_L3_bind.
+    rewrite translate_bind. rewrite bind_bind. rewrite bind_ret_l.
+    rewrite interp_cfg_to_L3_ret. rewrite translate_ret. rewrite bind_ret_l.
+    rewrite bind_ret_l. rewrite interp_cfg_to_L3_ret. rewrite translate_ret.
+    rewrite bind_ret_l.
+    (* END rewrite *)
     clear Heqi10. rewrite Heqi9.
     Transparent denote_terminator. cbn.
+
+    (* START rewrite *)
     rewrite translate_trigger. rewrite lookup_E_to_exp_E_Local.
     rewrite subevent_subevent. rewrite translate_bind.
     rewrite bind_bind. rewrite translate_trigger.
-    cbn... cbn.
+    rewrite interp_cfg_to_L3_bind.
+    rewrite translate_bind.
+    (* END rewrite *)
+    focus_single_step_v.
+
+    cbn...
+    cbn.
     2 : {
       setoid_rewrite lookup_alist_add_eq. reflexivity.
     }
 
     (* We find that k < n, thus we go back to looping on the body *)
+    match goal with
+    | [ |- context[(g, ?h)]] => remember h
+    end.
+    assert (Hequ' :u ≡ 'u_one). admit.
+    rewrite Hequ'.
     cbn...
-    rewrite eval_int_icmp_aux.
-    Typeclasses eauto := 4.
-    cbn...
-    focus_single_step_v.
-    Typeclasses eauto :=.
-    setoid_rewrite translate_ret.
-    setoid_rewrite interp_cfg_to_L3_ret.
-    rewrite translate_ret. rewrite bind_ret_l.
 
     rewrite Heqi11. cbn.
-    2 : admit. 2 : admit. (* TODO: Freshness *)
     cbn... clear Heqi11.
 
+
     (* Step 2 : Jump back to body_entry (since we have checked k < n). *)
-    unfold fmap, Fmap_block. cbn. rewrite convert_typ_block_app.
-    rewrite list_cons_app. rewrite denote_bks_unfold_in.
-    2 : { rewrite <- list_cons_app. setoid_rewrite find_block_eq. reflexivity. cbn. reflexivity.  }
-    cbn... rewrite denote_phi_tl. 2 : admit. (* TODO: Freshness *)
+    simpl. cbn...
+    simpl.
+    rewrite list_cons_app. cbn...
+
+    rewrite denote_bks_unfold_in.
+
+    2 : {
+      rewrite list_cons_app.
+      erewrite blk_id_norepet_find_block.
+      reflexivity. 2 : reflexivity.
+      red; cbn; rewrite map_app; cbn.
+      subst. cbn.
+      apply UNIQUE_IDENTS.
+      rewrite find_block_eq. reflexivity. subst. cbn. reflexivity.
+    }
+    cbn...
+    subst. cbn...
+    (* rewrite Heqb0_bk, Heqentry_bk, Heqloopcont_bk. cbn... *)
+    rewrite denote_phi_tl.
     focus_single_step_v.
+    2 : {
+      inversion UNIQUE_IDENTS.
+      cbn in H2. intro. subst. apply H1. right.
+      apply in_or_app. right. constructor. reflexivity.
+    }
     Transparent denote_phi. unfold denote_phi. rewrite assoc_hd. cbn.
     cbn... cbn. rewrite translate_ret. rewrite bind_ret_l.
     Opaque denote_phi.
     2 : {
-      setoid_rewrite lookup_alist_add_ineq. 2 : { admit. } (* TODO: Freshness *)
+      setoid_rewrite lookup_alist_add_ineq.
+      2 : { admit. } (* TODO: Freshness of local vars *)
       setoid_rewrite lookup_alist_add_eq. reflexivity.
     }
-    cbn... rewrite Heqi12. cbn...
+    cbn... rewrite Heqi7. cbn...
+
     (* Got the phi node from loop cont block, now! Time to jump to body_entry. *)
     (* Before that, we need to clean up some fluff. *)
-    cbn... focus_single_step_v.
-    rewrite interp_cfg_to_L3_LW. cbn.
-    rewrite translate_ret. rewrite bind_ret_l. rewrite Heqi13.
+    cbn... focus_single_step_v. cbn...
+    subst.
+    (* rewrite Heqi13. clear Heqi13. *)
 
-    focus_single_step_v. cbn...
-    rewrite Heqi14. clear Heqi13 Heqi14. clear i13 i14.
     cbn...
-    cbn. rewrite interp_cfg_to_L3_ret. setoid_rewrite translate_ret.
+    focus_single_step_v. cbn...
+    subst.
+    cbn...
+    cbn...
+    rewrite interp_cfg_to_L3_LW. cbn. setoid_rewrite translate_ret.
+    rewrite bind_ret_l.
+    cbn... cbn.
+    rewrite interp_cfg_to_L3_ret. setoid_rewrite translate_ret.
     rewrite bind_ret_l. rewrite interp_cfg_to_L3_bind.
     setoid_rewrite translate_ret. setoid_rewrite interp_cfg_to_L3_ret.
     rewrite bind_ret_l.
@@ -580,69 +654,89 @@ Proof with rauto.
     (* Starting to see body entry in the horizon. We need to apply the body hypothesis
        to retrieve the fact that "bks" entering from "body_entry" is the same denotation
        as "body_bks" entering from "body_entry". *)
-    match goal with
-    | [ |- context[denote_bks ?l]] => remember l as bks
-    end.
-    clear i11 i12 Heqi12 i10 i9 Heqi9. clear i7 Heqi7.
 
     (* Step 3 : Starting to think about applying body hypothesis *)
     (* Step 3.1 : Make right had side of equation agree with right hand side of HBODY *)
     match goal with
     | [ |- context[interp_cfg _ _ ?l _]] => remember l as LOCAL
     end.
-    match goal with
-    | [ |- eutt ?R _ _ ] => remember R as REL
-    end.
 
-    pose proof @rcompose_eq_r. specialize (H _ _ REL).
-    rewrite H.
+    assert (H0': (forall A (b : A) b1 l0 l1, b :: b1 :: l0 ++ l1 ≡ (b :: [b1]) ++ l0 ++ l1)%list). cbn. reflexivity.
+    rewrite H0'.
 
-    (* If we enter from body_entry, having either body_blocks or bks should be the same *)
-    eapply eqit_trans.
+    rewrite denote_bks_prefix_.
     2 : {
-      Unshelve.
-      2 : exact (with_err_LB (interp_cfg
-                                (denote_bks (convert_typ [ ] body_blocks)
-                                            (b0, body_entry)) g LOCAL mV)).
-      pose proof @body_blocks_from_entry_eq.
 
-      rewrite H0.
-      2 : {
-        Unshelve.
-        2 : exact prefix. 8 :exact n. 2 : exact loopvar. 2 : exact loopcontblock.
-        2 : exact nextblock. 2 : exact entry_id. 2 : exact s1. 2 : exact s2.
-        cbn. apply IN. auto.
-      }
-      (* rewrite Heqs. rewrite Heqs0. rewrite Heqs1. rewrite Heqs2. rewrite Heqs3. rewrite Heqs4. *)
-      (*   rewrite Heqs5. reflexivity. *)
-      (* } *)
-      subst.
-      rewrite list_cons_app.
-      cbn. unfold fmap, Fmap_block. cbn.
-
-      rewrite list_cons_app.
-
-      (* Ignore entry_id *)
-      rewrite denote_bks_flow_right. 2 : admit. 2 : admit. (* TODO: Freshness *)
-      cbn... cbn.
-      unfold fmap, Fmap_block. cbn.
-      cbn...
-      admit.
-      (* reflexivity. *)
-      admit. (* *)
+        assert (forall bs, map blk_id bs ≡ map blk_id (convert_typ [] bs)). {
+        induction bs. cbn. reflexivity.
+        cbn. rewrite IHbs. reflexivity.
+        }
+      subst. rewrite <-H. unfold block_ids in IN. apply IN.
     }
 
-    (* Now the RHS is the same as the body hypothesis, we should now reduce the LHS respectively. *)
-    unfold build_vec_gen, build_vec_gen_aux. cbn.
-    assert (n - S (n - S k) ≡ k).
-    assert (n - S (n - S k) ≡ n - (1 + (n - 1 - k))) by lia.
+    2 : {
+      subst. cbn. rewrite map_app. cbn. apply UNIQUE_IDENTS.
+    }
+    cbn...
+
+
+    assert (n - S k > 1). admit.
+    assert (n - S k ≡ S (n - S (S k))). lia.
+
+    rewrite H0.
+    eapply eutt_clo_bind.
 
     (* Step 3 (Actually applying BH): By body hypothesis, this will lead to my invariant being true at
        step S k, and to jumping to loopcontblock. *)
+    eapply HBODY.
+    
+    red. split.
+    eapply STABLE. apply INV.
+    (*TODO: Local var alist unique *) admit.
+    subst. 
+
+    cbn.
+    (* admit (* TODO: fix k in L316 to (S k) *). *)
+    assert (H3 : loopvar ≡ loopvar) by reflexivity.
+    subst.
+    eapply rel_dec_eq_true in H3. cbn. rewrite H3.
+    assert (ARITH: UVALUE_I64 ((int64) ((Z) (n - S (S k) - 1)) + (int64) 1) ≡ uvalue_of_nat (n - S (S k))).
+    admit.
+    rewrite ARITH.
+    auto.
+    typeclasses eauto.
+
+    intros *. destruct u1, u2. destruct p. destruct p.
+    intros (LOOPVAR' & HS & IH').
+    rewrite HS.
 
     (* Step 4 : Back to starting from loopcontblock and have reestablished everything at the next index:
-       conclude by IH *)
-
+        conclude by IH *)
+    assert (EQ' : S (S (n - S (S k))) ≡ n - k). lia.
+    rewrite EQ'. subst. cbn in IH. rewrite convert_typ_block_app in IH. cbn in IH.
+      match goal with
+      | [ |- context[denote_bks (?a :: ?b :: ?c ++ ?d)]] => remember a; remember b; remember c; remember d
+      end.
+      match goal with
+      | [ H : context[denote_bks (?a :: ?b :: ?c ++ ?d)] |- _] => remember a; remember b; remember c; remember d
+      end
+      .
+      assert (EQB1: b2 ≡ b). {
+        subst.
+        rewrite 2 typ_to_dtyp_I. reflexivity.
+      }
+      assert (EQB2: b3 ≡ b1). {
+        subst. rewrite typ_to_dtyp_I. reflexivity.
+      }
+      assert (EQB3 : l4 ≡ l2). {
+        subst. rewrite 2 typ_to_dtyp_I. reflexivity.
+      }
+      rewrite <- EQB1,<- EQB2,<- EQB3.
+      eapply IH. lia. lia.
+      split.
+      assert (S (n - S (S k)) ≡ n - S k). lia. rewrite <- H1. auto.
+      assert (n - S (S k) ≡ n - S k - 1) by lia.
+      rewrite <- H1. auto. Unshelve. auto.
 Admitted.
 
 
